dimsum_examples/iris/rec.v
@@ -1,3 +1,4 @@
+From iris.algebra Require Import big_op gmap frac agree dfrac_agree.
 From iris.base_logic.lib Require Import ghost_map.
 From dimsum.core.iris Require Export iris.
 From dimsum.examples Require Export rec.
@@ -7,23 +8,30 @@ Set Default Proof Using "Type".
 
 Local Open Scope Z_scope.
 
+Definition fnsUR : cmra :=
+  agreeR (gmapO string (leibnizO fndef)).
+
+Definition to_fns : gmap string fndef → fnsUR :=
+  to_agree.
+
+
 Class recPreGS (Σ : gFunctors) := RecPreGS {
-  rec_heap_ghost_map_preG :> ghost_mapG Σ loc val;
-  rec_alloc_ghost_map_preG :> ghost_mapG Σ prov nat;
-  rec_fn_ghost_map_preG :> ghost_mapG Σ string fndef;
+  rec_mapsto_ghost_map_preG :> ghost_mapG Σ loc val;
+  rec_alloc_ghost_map_preG :> ghost_mapG Σ loc Z;
+  rec_fn_preG :> inG Σ fnsUR;
 }.
 
 Class recGS (Σ : gFunctors) := RecGS {
-  rec_heap_ghost_mapG :> ghost_mapG Σ loc val;
-  rec_alloc_ghost_mapG :> ghost_mapG Σ prov nat;
-  rec_fn_ghost_mapG :> ghost_mapG Σ string fndef;
-  rec_heap_name : gname;
+  rec_mapsto_ghost_mapG :> ghost_mapG Σ loc val;
+  rec_alloc_ghost_mapG :> ghost_mapG Σ loc Z;
+  rec_fnG :> inG Σ fnsUR;
+  rec_mapsto_name : gname;
   rec_alloc_name : gname;
   rec_fn_name : gname;
 }.
 
 Definition recΣ : gFunctors :=
-  #[ ghost_mapΣ loc val; ghost_mapΣ prov nat; ghost_mapΣ string fndef ].
+  #[ ghost_mapΣ loc val; ghost_mapΣ loc Z; GFunctor fnsUR ].
 
 Global Instance subG_recΣ Σ :
   subG recΣ Σ → recPreGS Σ.
@@ -33,7 +41,7 @@ Section definitions.
   Context `{!recGS Σ}.
 
   Definition rec_mapsto_def (l : loc) (q : dfrac) (v : val) : iProp Σ :=
-    ghost_map_elem rec_heap_name l q v.
+    ghost_map_elem rec_mapsto_name l q v.
   Local Definition rec_mapsto_aux : seal (@rec_mapsto_def).
   Proof. by eexists. Qed.
   Definition rec_mapsto := rec_mapsto_aux.(unseal).
@@ -41,21 +49,34 @@ Section definitions.
     @rec_mapsto = @rec_mapsto_def := rec_mapsto_aux.(seal_eq).
 
   Definition rec_mapsto_auth (h : gmap loc val) : iProp Σ :=
-    ghost_map_auth rec_heap_name 1 h.
+    ghost_map_auth rec_mapsto_name 1 h.
 
-  Definition rec_fn_mapsto_def (f : string) (fn : fndef) : iProp Σ :=
-    ghost_map_elem rec_fn_name f DfracDiscarded fn.
+  Definition rec_alloc_def (l : loc) (sz : Z) : iProp Σ :=
+    ghost_map_elem rec_alloc_name l (DfracOwn 1) sz.
+  Local Definition rec_alloc_aux : seal (@rec_alloc_def).
+  Proof. by eexists. Qed.
+  Definition rec_alloc := rec_alloc_aux.(unseal).
+  Local Definition rec_alloc_unseal :
+    @rec_alloc = @rec_alloc_def := rec_alloc_aux.(seal_eq).
+
+  Definition rec_alloc_auth (h : gset loc) : iProp Σ :=
+    ∃ p,
+    ⌜∀ l sz, p !! l = Some sz → sz > 0⌝ ∗
+    ⌜∀ l sz, p !! l = Some sz → ∀ l', l'.1 = l.1 → l' ∈ h ↔ l.2 ≤ l'.2 < l.2 + sz⌝ ∗
+    ghost_map_auth rec_alloc_name 1 p.
+
+  Definition rec_fn_auth (fns : gmap string fndef) : iProp Σ :=
+    own rec_fn_name (to_fns fns).
+  Definition rec_fn_mapsto_def (f : string) (fn : option fndef) : iProp Σ :=
+    ∃ fns, ⌜fns !! f = fn⌝ ∗ rec_fn_auth fns.
   Local Definition rec_fn_mapsto_aux : seal (@rec_fn_mapsto_def).
   Proof. by eexists. Qed.
   Definition rec_fn_mapsto := rec_fn_mapsto_aux.(unseal).
   Local Definition rec_fn_mapsto_unseal :
     @rec_fn_mapsto = @rec_fn_mapsto_def := rec_fn_mapsto_aux.(seal_eq).
 
-  Definition rec_fn_auth (fns : gmap string fndef) : iProp Σ :=
-    ghost_map_auth rec_fn_name 1 fns.
-
   Definition rec_state_interp (σ : rec_state) : iProp Σ :=
-    rec_mapsto_auth (h_heap (st_heap σ)) ∗ rec_fn_auth (st_fns σ).
+    rec_mapsto_auth (h_heap (st_heap σ)) ∗ rec_alloc_auth (dom (h_heap (st_heap σ))) ∗ rec_fn_auth (st_fns σ).
 End definitions.
 
 Notation "l ↦ v" := (rec_mapsto l (DfracOwn 1) v)
@@ -65,42 +86,85 @@ Notation "f ↪ fn" := (rec_fn_mapsto f fn)
 
 Local Ltac unseal := rewrite
   ?rec_mapsto_unseal /rec_mapsto_def /rec_mapsto_auth
+  ?rec_alloc_unseal /rec_alloc_def /rec_alloc_auth
   ?rec_fn_mapsto_unseal /rec_fn_mapsto_def /rec_fn_auth.
 
 Section lemmas.
   Context `{!recGS Σ}.
 
+  Global Instance rec_fn_auth_pers fns : Persistent (rec_fn_auth fns).
+  Proof. unseal. apply _. Qed.
+
   Global Instance rec_fn_mapsto_pers f fn : Persistent (f ↪ fn).
   Proof. unseal. apply _. Qed.
 
+  Lemma rec_fn_auth_agree fns1 fns2 :
+    rec_fn_auth fns1 -∗ rec_fn_auth fns2 -∗ ⌜fns1 = fns2⌝.
+  Proof.
+    unseal. iIntros "H1 H2".
+    iDestruct (own_valid_2 with "H1 H2") as %Hvalid.
+    move: Hvalid => /to_agree_op_valid.
+    by fold_leibniz.
+  Qed.
+
   Lemma rec_fn_lookup f fn fns :
-    rec_fn_auth fns -∗ f ↪ fn -∗ ⌜fns !! f = Some fn⌝.
-  Proof. unseal. apply ghost_map_lookup. Qed.
+    rec_fn_auth fns -∗ f ↪ fn -∗ ⌜fns !! f = fn⌝.
+  Proof.
+    unseal. iIntros "Htbl Hf".
+    iDestruct "Hf" as (fns2 ?) "Hf".
+    by iDestruct (rec_fn_auth_agree with "Htbl Hf") as %->.
+  Qed.
 
 End lemmas.
 
-Program Canonical Structure rec_mod_lang {Σ} `{!recGS Σ} := {| (*  *)
-  mexpr := expr;
+Lemma recgs_alloc `{!recPreGS Σ} fns :
+  ⊢ |==> ∃ H : recGS Σ, rec_mapsto_auth ∅ ∗ rec_alloc_auth ∅ ∗ rec_fn_auth fns.
+Proof.
+  iMod (own_alloc (to_fns fns)) as (γf) "#Hfns" => //.
+  iMod (ghost_map_alloc (V:=val)) as (γh) "[??]".
+  iMod (ghost_map_alloc (V:=Z)) as (γa) "[??]".
+
+  iModIntro. iExists (RecGS _ _ _ _ γh γa γf). iFrame "#∗".
+  iExists ∅. iFrame. iPureIntro; split!.
+Qed.
+
+Record expr_heap := ExprHeap {
+ eh_expr : expr;
+ eh_heap : option heap_state;
+}.
+Add Printing Constructor expr_heap.
+
+Definition expr_heap_fill (K : list expr_ectx) (e : expr_heap) : expr_heap :=
+  ExprHeap (expr_fill K (eh_expr e)) (eh_heap e).
+
+Arguments expr_heap_fill !_ _ /.
+
+Notation "e @ h" := (ExprHeap e (Some h)) (at level 14) : stdpp_scope.
+Notation "e @ -" := (ExprHeap e None) (at level 14, only parsing) : stdpp_scope.
+Notation "e" := (ExprHeap e None) (at level 14, only printing) : stdpp_scope.
+
+Program Canonical Structure rec_mod_lang {Σ} `{!recGS Σ} := {|
+  mexpr := expr_heap;
   mectx := list expr_ectx;
-  mfill := expr_fill;
+  mfill := expr_heap_fill;
   mcomp_ectx := flip app;
   mtrans := rec_trans;
-  mexpr_rel σ e := e = st_expr σ;
+  mexpr_rel σ e := eh_expr e = st_expr σ ∧ if eh_heap e is Some h then h = st_heap σ else True;
   mstate_interp := rec_state_interp;
 |}.
-Next Obligation. move => *. by rewrite expr_fill_app. Qed.
+Next Obligation. move => ???? [??]/=. by rewrite /expr_heap_fill/= expr_fill_app. Qed.
 
 Section lifting.
   Context `{!dimsumGS Σ} `{!recGS Σ}.
 
   Lemma sim_rec_Call_internal f fn es Π Φ vs `{!AsVals es vs None} :
     length vs = length (fd_args fn) →
-    f ↪ fn -∗
-    ▷ₒ Φ (AllocA fn.(fd_vars) (subst_l fn.(fd_args) vs fn.(fd_body))) Π -∗
-    TGT Call f es [{ Π }] {{ Φ }}.
+    f ↪ Some fn -∗
+    ▷ₒ Φ (AllocA fn.(fd_vars) (subst_l fn.(fd_args) vs fn.(fd_body)) @ -) Π -∗
+    TGT Call f es @ - [{ Π }] {{ Φ }}.
   Proof.
     destruct AsVals0. iIntros (?) "Hfn HΦ".
-    iApply sim_tgt_expr_step_None => /=. iIntros (? [e h fns] ??? Hp) "[Hh Hfns]". simplify_eq/=.
+    iApply sim_tgt_expr_step_None => /=. iIntros (? [e h fns] ?? [??] Hp) "[Hh [Ha Hfns]]". simplify_eq/=.
     iDestruct (rec_fn_lookup with "[$] [$]") as %?.
     rewrite right_id_L in Hp.
     exploit prim_step_inv_head; [done|..].
@@ -108,8 +172,8 @@ Section lifting.
       move => /= ??? e' [_ Heq]. by apply: list_expr_val_inv. }
     { done. }
     move => [? [Hstep ?]]. inv Hstep.
-    do 2 iModIntro. iSplit!. iFrame.
-    by iApply sim_tgt_expr_stop.
+    do 2 iModIntro. iExists _, (_ @ -). iSplit!. iFrame.
+    by iApply sim_tgt_expr_stop2.
   Qed.
 End lifting.
 
@@ -122,41 +186,42 @@ Section memmove.
     d' = (if bool_decide (o = 1) then d else d +ₗ (- n + 1)) →
     s' = (if bool_decide (o = 1) then s else s +ₗ (- n + 1)) →
     (if bool_decide (o = 1) then d.1 = s.1 → d.2 ≤ s.2 else d.1 = s.1 → s.2 ≤ d.2) →
-    "memcpy" ↪ memcpy_rec -∗
+    "memcpy" ↪ Some memcpy_rec -∗
     ([∗ list] i↦v∈hvs, (s' +ₗ i) ↦ v) -∗
     ([∗ list] i↦_∈hvs, ∃ v, (d' +ₗ i) ↦ v) -∗
-    (([∗ list] i↦v∈hvs, (s' +ₗ i) ↦ v) -∗ ([∗ list] i↦v∈hvs, (d' +ₗ i) ↦ v) -∗ Φ (Val 0) Π) -∗
-    TGT Call "memcpy" [Val (ValLoc d); Val $ ValLoc s; Val $ ValNum n; Val $ ValNum o] [{ Π }] {{ Φ }}.
+    (([∗ list] i↦v∈hvs, (s' +ₗ i) ↦ v) -∗ ([∗ list] i↦v∈hvs, (d' +ₗ i) ↦ v) -∗ Φ (Val 0 @ -) Π) -∗
+    TGT Call "memcpy" [Val (ValLoc d); Val $ ValLoc s; Val $ ValNum n; Val $ ValNum o] @ - [{ Π }] {{ Φ }}.
   Proof.
     iIntros (Hn Ho Hd' Hs' Hle) "#Hf Hs Hd HΦ".
     iApply sim_tgt_expr_ctx. iIntros "#?".
     iRevert (d d' s s' n hvs Hn Hd' Hs' Hle) "Hs Hd HΦ".
     iApply ord_loeb; [done|].
     iIntros "!> #-#IH" (d d' s s' n hvs Hn Hd' Hs' Hle) "Hs Hd HΦ". simplify_eq.
-    iApply (sim_tgt_expr_bind []).
+    iApply (sim_tgt_expr_bind [] (_ @ -) with "[-]").
     iApply (sim_rec_Call_internal with "Hf"); [done|]. iModIntro => /=.
   Abort.
 
   Lemma sim_memmove Π Φ d s n hvs :
     n = Z.of_nat (length hvs) →
-    "memmove" ↪ memmove_rec -∗
-    "memcpy" ↪ memcpy_rec -∗
+    "memmove" ↪ Some memmove_rec -∗
+    "memcpy" ↪ Some memcpy_rec -∗
     □ (∀ l1 l2 Φ,
-        (∀ b, ⌜l1.1 = l2.1 → b = bool_decide (l1.2 ≤ l2.2)⌝ -∗ Φ (Val (ValBool b)) Π) -∗
-          TGT Call "locle" [Val (ValLoc l1); Val $ ValLoc l2] [{ Π }] {{ Φ }}) -∗
+        (∀ b, ⌜l1.1 = l2.1 → b = bool_decide (l1.2 ≤ l2.2)⌝ -∗ Φ (Val (ValBool b) @ -) Π) -∗
+          TGT Call "locle" [Val (ValLoc l1); Val $ ValLoc l2] @ - [{ Π }] {{ Φ }}) -∗
     ([∗ list] i↦v∈hvs, (s +ₗ i) ↦ v) -∗
     ([∗ list] i↦_∈hvs, ∃ v, (d +ₗ i) ↦ v) -∗
-    (([∗ list] i↦v∈hvs, (s +ₗ i) ↦ v) -∗ ([∗ list] i↦v∈hvs, (d +ₗ i) ↦ v) -∗ Φ (Val 0) Π) -∗
-    TGT Call "memmove" [Val (ValLoc d); Val $ ValLoc s; Val $ ValNum n] [{ Π }] {{ Φ }}.
+    (([∗ list] i↦v∈hvs, (s +ₗ i) ↦ v) -∗ ([∗ list] i↦v∈hvs, (d +ₗ i) ↦ v) -∗ Φ (Val 0 @ -) Π) -∗
+    TGT Call "memmove" [Val (ValLoc d); Val $ ValLoc s; Val $ ValNum n] @ - [{ Π }] {{ Φ }}.
   Proof.
     iIntros (->) "#Hmemmove #Hmemcpy #Hlocle Hs Hd HΦ".
-    iApply (sim_tgt_expr_bind []).
+    iApply (sim_tgt_expr_bind [] (_ @ -)).
     iApply (sim_rec_Call_internal with "Hmemmove"); [done|]. iModIntro => /=.
+    simpl.
   Abort.
 
   Lemma sim_locle Π Φ l1 l2 :
-    (∀ b, ⌜l1.1 = l2.1 → b = bool_decide (l1.2 ≤ l2.2)⌝ -∗ Φ (Val (ValBool b)) Π) -∗
-    TGT Call "locle" [Val (ValLoc l1); Val $ ValLoc l2] [{ Π }] {{ Φ }}.
+    (∀ b, ⌜l1.1 = l2.1 → b = bool_decide (l1.2 ≤ l2.2)⌝ -∗ Φ (Val (ValBool b) @ -) Π) -∗
+    TGT Call "locle" [Val (ValLoc l1); Val $ ValLoc l2] @ - [{ Π }] {{ Φ }}.
   Proof. Admitted.
 
 
@@ -165,230 +230,21 @@ End memmove.
 Section sim.
   Context {Σ : gFunctors} {EV : Type} `{!dimsumGS Σ}.
 
-  Definition sim_tgt_handler (m_t m_s : mod_trans EV)
-    (Π_s : (option EV → m_state m_s → iProp Σ) → iProp Σ) :
+  Definition sim_tgt_handler {m_t m_s : mod_trans EV}
+    (σ : m_state m_s) :
     option EV → ((m_state m_t → iProp Σ) → iProp Σ) → iProp Σ :=
-    λ κ Pσ, (Π_s (λ κ' σ_s', ⌜κ = κ'⌝ ∗ Pσ (λ σ_t', σ_t' ⪯{m_t, m_s} σ_s')))%I.
+    λ κ Pσ, (σ ≈{m_s}≈>ₛ (λ κ' σ_s', ⌜κ = κ'⌝ ∗ Pσ (λ σ_t', σ_t' ⪯{m_t, m_s} σ_s')))%I.
 
   Lemma sim_tgt_handler_intro m_t m_s σ_t σ_s :
-    σ_t ≈{m_t}≈>ₜ sim_tgt_handler m_t m_s (sim_src m_s σ_s) -∗ σ_t ⪯{m_t, m_s} σ_s.
-  Proof. Admitted.
+    σ_t ≈{m_t}≈>ₜ sim_tgt_handler σ_s -∗ σ_t ⪯{m_t, m_s} σ_s.
+  Proof.
+    iIntros "?". rewrite sim_unfold.
+    iApply (sim_tgt_wand with "[$]"). iIntros (??) "?".
+    iApply (sim_src_wand with "[$]"). iIntros (??) "[% ?]".
+    iSplit; [done|]. by iApply bi_mono1_intro0.
+  Qed.
+
 End sim.
-
-From dimsum.core Require Import product.
-
-Section map.
-  Context {Σ : gFunctors} {EV1 EV2 : Type} {S : Type} `{!dimsumGS Σ}.
-  Implicit Types (f : map_mod_fn EV1 EV2 S).
-
-  Lemma sim_tgt_map m f σ σf Π :
-    (σ ≈{m}≈>ₜ λ κ Pσ,
-      ∀ κ' σf' ok, ⌜if κ is Some e then f σf e κ' σf' ok else κ' = None ∧ σf' = σf ∧ ok = true⌝ -∗
-         Π κ' (λ P, Pσ (λ σ', P (σ', (σf', ok))))) -∗
-    (σ, (σf, true)) ≈{map_trans m f}≈>ₜ Π.
-  Proof.
-    iIntros "Hsim".
-    pose (F := (λ σ Π', (∀ κ Pσ, Π' κ Pσ -∗
-         ∀ κ' σf' ok, ⌜if κ is Some e then f σf e κ' σf' ok else κ' = None ∧ σf' = σf ∧ ok = true⌝ -∗
-          Π κ' (λ P, Pσ (λ σ', P (σ', (σf', ok))))) -∗ (σ, (σf, true)) ≈{map_trans m f}≈>ₜ Π)%I).
-    iAssert (∀ Π, σ ≈{ m }≈>ₜ Π -∗ F σ Π)%I as "Hgen"; last first.
-    { iApply ("Hgen" with "Hsim"). iIntros (??) "?". done. }
-    iIntros (?) "Hsim".
-    iApply (sim_tgt_ind with "[] Hsim"). { solve_proper. }
-    iIntros "!>" (??) "Hsim". iIntros "Hc".
-    iApply (sim_tgt_ctx with "[-]"). iIntros "?".
-    iApply (sim_tgt_bi_mono1 with "[-]").
-    iApply (fupd_sim_tgt with "[-]").
-    iMod ("Hsim" with "[$]") as "[[% [? HP]]| Hs ]". {
-      iModIntro. iDestruct ("Hc" with "[$] [//]") as "Hc".
-      iApply (sim_tgt_stop with "[-]").
-      iApply (bi_mono1_intro with "Hc"). iIntros (?) "?".
-      iDestruct ("HP" with "[$]") as "$".
-    }
-    iModIntro. iApply (sim_tgt_step with "[-]"). iIntros (?? Hstep). inv_all/= @m_step.
-    all: iMod ("Hs" with "[//]") as "Hs"; do 2 iModIntro.
-    - do 2 case_match; simplify_eq. iDestruct "Hs" as "[[% [? HP]]|[%[%[% HF]]]]".
-      + iDestruct ("Hc" with "[$] [//]") as "Hc".
-        iLeft. iApply (bi_mono1_intro with "Hc"). iIntros (?) "?".
-        iDestruct ("HP" with "[$]") as (??) "?".
-        iExists (_, _). iFrame. iSplit!.
-      + iRight. iExists (_, _). iSplit!; [done|].
-        iApply (sim_tgt_wand with "[-] []"); [by iApply "HF"|].
-        iIntros (??) "HΠ". by iApply bi_mono1_intro'.
-    - iDestruct "Hs" as "[[% [? HP]]|[%[%[% HF]]]]"; simplify_eq.
-      iDestruct ("Hc" with "[$] [//]") as "Hc".
-      iLeft. iExists _. iFrame. iIntros (?) "?".
-      iDestruct ("HP" with "[$]") as (??) "?".
-      iExists (_, _). iFrame. iSplit!.
-  Qed.
-
-  Lemma sim_src_map m f σ σf Π `{!VisNoAng m} :
-    (σ ≈{m}≈>ₛ λ κ σ',
-      ∃ κ' σf' ok, ⌜if κ is Some e then f σf e κ' σf' ok else κ' = None ∧ σf' = σf ∧ ok = true⌝ ∗
-         Π κ' (σ', (σf', ok))) -∗
-    (σ, (σf, true)) ≈{map_trans m f}≈>ₛ Π.
-  Proof.
-    iIntros "Hsim".
-    pose (F := (λ σ Π', (∀ κ σ', Π' κ σ' -∗
-         ∃ κ' σf' ok, ⌜if κ is Some e then f σf e κ' σf' ok else κ' = None ∧ σf' = σf ∧ ok = true⌝ ∗
-          Π κ' (σ', (σf', ok))) -∗ (σ, (σf, true)) ≈{map_trans m f}≈>ₛ Π)%I).
-    iAssert (∀ Π, σ ≈{ m }≈>ₛ Π -∗ F σ Π)%I as "Hgen"; last first.
-    { iApply ("Hgen" with "Hsim"). iIntros (??) "?". done. }
-    iIntros (?) "Hsim".
-    iApply (sim_src_ind with "[] Hsim"). { solve_proper. }
-    iIntros "!>" (??) "Hsim". iIntros "Hc".
-    iApply (sim_src_ctx with "[-]"). iIntros "?".
-    iApply (fupd_sim_src with "[-]").
-    iMod ("Hsim" with "[$]") as "[?| [%κ [% [% Hs]]] ]". {
-      iModIntro. iApply (sim_src_stop with "[-]").
-      iDestruct ("Hc" with "[$]") as (???[?[??]]) "Hc". by simplify_eq.
-    }
-    destruct κ.
-    - exploit vis_no_all; [done|] => -[σ'' ?].
-      iMod ("Hs" with "[%]") as "Hs"; [naive_solver|]. iModIntro.
-      iDestruct ("Hc" with "[$]") as (????) "Hs".
-      iApply (sim_src_step_end with "[-]"). { econs. { apply: ProductStepBoth; [done|]. by econs. } done. }
-      iIntros ([σ' ?] [??]) "!>". have ? : σ' = σ'' by naive_solver. by simplify_eq.
-    - iModIntro. iApply (sim_src_step with "[-]"). { econs; [by econs|done]. }
-      iIntros ([??][??]). simplify_eq. iMod ("Hs" with "[//]") as "HF". iModIntro.
-      by iApply "HF".
-  Qed.
-End map.
-
-From dimsum.core Require Import state_transform.
-
-Section state_transform.
-  Context {Σ : gFunctors} {EV : Type} {S : Type} `{!dimsumGS Σ}.
-
-  Lemma sim_tgt_state_transform (m : mod_trans EV) σ' (R : S → m.(m_state) → Prop) σ Π :
-   (∀ σ σ1 σ2, R σ σ1 → R σ σ2 → σ1 = σ2) →
-   (∀ σ1 σ σ' κ Pσ, m_step m σ κ Pσ → Pσ σ' → R σ1 σ → ∃ σ'', R σ'' σ') →
-   R σ σ' →
-   (σ' ≈{m}≈>ₜ λ κ Pσ, Π κ (λ P, Pσ (λ σ'', ∀ σ''', ⌜R σ''' σ''⌝ -∗ P σ'''))) -∗
-    σ ≈{state_transform_trans m R}≈>ₜ Π.
-  Proof.
-    iIntros (Heq HRstep HR) "Hsim".
-    pose (F := (λ σ' Π', ∀ σ,
-                   ⌜R σ σ'⌝ -∗
-                   (∀ κ Pσ, Π' κ Pσ -∗ Π κ (λ P, Pσ (λ σ'', ∀ σ''', ⌜R σ''' σ''⌝ -∗ P σ'''))) -∗
-                   σ ≈{state_transform_trans m R}≈>ₜ Π)%I).
-    iAssert (∀ Π, σ' ≈{ m }≈>ₜ Π -∗ F σ' Π)%I as "Hgen"; last first.
-    { iApply ("Hgen" with "Hsim"); [done|]. iIntros (??) "?". done. }
-    iIntros (?) "Hsim".
-    iApply (sim_tgt_ind with "[] Hsim"). { solve_proper. }
-    clear σ' σ HR. iIntros "!>" (σ'?) "Hsim". iIntros (σ HR) "Hc".
-    iApply (sim_tgt_ctx with "[-]"). iIntros "?".
-    iApply (sim_tgt_bi_mono1 with "[-]").
-    iApply (fupd_sim_tgt with "[-]").
-    iMod ("Hsim" with "[$]") as "[[% [HΠ HP]]| Hs ]". {
-      iModIntro. iApply (sim_tgt_stop with "[-]").
-      iApply (bi_mono1_intro with "[Hc HΠ]"); [by iApply "Hc"|] => /=.
-      iIntros (?) "?". iDestruct ("HP" with "[$]") as "HP". by iApply "HP".
-    }
-    iModIntro. iApply (sim_tgt_step with "[-]"). iIntros (?? Hstep). inv_all/= @m_step.
-    have ?: σ' = σ'0 by naive_solver. subst.
-    iMod ("Hs" with "[//]") as "Hs"; do 2 iModIntro.
-    iDestruct "Hs" as "[[% [? HP]]|[%[%[% HF]]]]".
-    - iDestruct ("Hc" with "[$]") as "Hc".
-      iLeft. iApply (bi_mono1_intro with "Hc"). iIntros (?) "?".
-      iDestruct ("HP" with "[$]") as (??) "HP".
-      exploit HRstep; [done..|] => -[??].
-      iSplit!; [done..|]. by iApply "HP".
-    - iRight. simplify_eq. exploit HRstep; [done..|] => -[??].
-      iSplit!; [done..|]. iApply (sim_tgt_wand with "[-] []"); [by iApply "HF"|].
-      iIntros (??) "HΠ". by iApply bi_mono1_intro'.
-  Qed.
-
-  Lemma sim_src_state_transform (m : mod_trans EV) σ' (R : S → m.(m_state) → Prop) σ Π :
-   R σ σ' →
-   (σ' ≈{m}≈>ₛ λ κ σ'', ∀ σ''', ⌜R σ''' σ''⌝ -∗ Π κ σ''') -∗
-    σ ≈{state_transform_trans m R}≈>ₛ Π.
-  Proof.
-    iIntros (HR) "Hsim".
-    pose (F := (λ σ' Π', ∀ σ,
-                   ⌜R σ σ'⌝ -∗
-                   (∀ κ σ'', Π' κ σ'' -∗ ∀ σ''', ⌜R σ''' σ''⌝ -∗ Π κ σ''') -∗
-                   σ ≈{state_transform_trans m R}≈>ₛ Π)%I).
-    iAssert (∀ Π, σ' ≈{ m }≈>ₛ Π -∗ F σ' Π)%I as "Hgen"; last first.
-    { iApply ("Hgen" with "Hsim"); [done|]. iIntros (??) "?". done. }
-    iIntros (?) "Hsim".
-    iApply (sim_src_ind with "[] Hsim"). { solve_proper. }
-    clear σ' σ HR. iIntros "!>" (σ'?) "Hsim". iIntros (σ HR) "Hc".
-    iApply (sim_src_ctx with "[-]"). iIntros "?".
-    iApply (fupd_sim_src with "[-]").
-    iMod ("Hsim" with "[$]") as "[?| [%κ [% [% Hs]]] ]". {
-      iModIntro. iApply (sim_src_stop with "[-]"). by iApply ("Hc" with "[$]").
-    }
-    iModIntro. iApply (sim_src_step with "[-]"); [by econs|].
-    iIntros (? [?[??]]). iMod ("Hs" with "[//]") as "Hs". iModIntro.
-    case_match.
-    - by iApply ("Hc" with "Hs").
-    - by iApply ("Hs" with "[//]").
-  Qed.
-End state_transform.
-
-From dimsum.core Require Import seq_product.
-
-Section seq_product.
-  Context {Σ : gFunctors} {EV : Type} `{!dimsumGS Σ}.
-
-  Lemma sim_tgt_seq_product_None (m1 m2 : mod_trans EV) σ1 σ2 Π :
-    (∀ p, ▷ₒ Π (Some (SPENone p)) (λ P, P (p, σ1, σ2))) -∗
-    (SPNone, σ1, σ2) ≈{seq_product_trans m1 m2}≈>ₜ Π.
-  Proof.
-    iIntros "HΠ". iApply (sim_tgt_bi_mono with "[-]").
-    iApply (sim_tgt_step_end with "[-]"). iIntros (???). inv_all @m_step. iSpecialize ("HΠ" $! _).
-    do 2 iModIntro. iApply (bi_mono1_intro with "HΠ"). iIntros (?) "?".
-    iApply bi_mono1_intro'. iSplit!.
-  Qed.
-
-  Lemma sim_src_seq_product_None p (m1 m2 : mod_trans EV) σ1 σ2 Π :
-    Π (Some (SPENone p)) (p, σ1, σ2) -∗
-    (SPNone, σ1, σ2) ≈{seq_product_trans m1 m2}≈>ₛ Π.
-  Proof.
-    iIntros "HΠ". iApply (sim_src_step_end with "[-]"); [by econs|].
-    iIntros (??). by simplify_eq.
-  Qed.
-
-  Lemma sim_tgt_seq_product_left (m1 m2 : mod_trans EV) σ1 σ2 Π :
-    (σ1 ≈{m1}≈>ₜ λ κ Pσ,
-      ∀ s', ⌜if κ is None then s' = SPLeft else True⌝ -∗
-         Π ((λ e, SPELeft e s') <$> κ) (λ P, Pσ (λ σ', P (s', σ', σ2)))) -∗
-    (SPLeft, σ1, σ2) ≈{seq_product_trans m1 m2}≈>ₜ Π.
-  Proof.
-    iIntros "Hsim".
-    pose (F := (λ σ Π', (∀ κ Pσ, Π' κ Pσ -∗
-         ∀ s', ⌜if κ is None then s' = SPLeft else True⌝ -∗
-         Π ((λ e, SPELeft e s') <$> κ) (λ P, Pσ (λ σ', P (s', σ', σ2)))) -∗
-         (SPLeft, σ, σ2) ≈{seq_product_trans m1 m2}≈>ₜ Π)%I).
-    iAssert (∀ Π, σ1 ≈{ m1 }≈>ₜ Π -∗ F σ1 Π)%I as "Hgen"; last first.
-    { iApply ("Hgen" with "Hsim"). iIntros (??) "?". done. }
-    iIntros (?) "Hsim".
-    iApply (sim_tgt_ind with "[] Hsim"). { solve_proper. }
-    iIntros "!>" (??) "Hsim". iIntros "Hc".
-    iApply (sim_tgt_ctx with "[-]"). iIntros "?".
-    iApply (sim_tgt_bi_mono1 with "[-]").
-    iApply (fupd_sim_tgt with "[-]").
-    iMod ("Hsim" with "[$]") as "[[% [? HP]]| Hs ]". {
-      iModIntro. iDestruct ("Hc" with "[$] [//]") as "Hc".
-      iApply sim_tgt_stop.
-      iApply (bi_mono1_intro with "[Hc] [-]"); [done|].
-      iIntros (?) "?". by iDestruct ("HP" with "[$]") as "HP".
-    }
-    iModIntro. iApply (sim_tgt_step with "[-]"). iIntros (?? Hstep). inv_all/= @m_step.
-    iMod ("Hs" with "[//]") as "Hs"; do 2 iModIntro.
-    iDestruct "Hs" as "[[% [? HP]]|[%[%[% HF]]]]"; simplify_eq/=.
-    - iDestruct ("Hc" with "[$] [//]") as "Hc".
-      iLeft. iApply (bi_mono1_intro with "Hc").
-      iIntros (?) "?".
-      iDestruct ("HP" with "[$]") as (??) "?".
-      iExists (_, _, _). iSplit!; [done|]. by iFrame.
-    - iRight. iExists (_, _, _). iSplit!; [done|].
-      iApply (sim_tgt_wand with "[-] []"); [by iApply "HF"|].
-      iIntros (??) "HΠ". by iApply bi_mono1_intro'.
-  Qed.
-
-End seq_product.
 
 Section link.
   Context {Σ : gFunctors} {EV : Type} {S : Type} `{!dimsumGS Σ}.
@@ -402,13 +258,13 @@ Section link.
   Proof.
     iIntros "HΠ".
     iApply (sim_tgt_bi_mono1 with "[-]").
-    iApply sim_tgt_state_transform; [naive_solver| admit |done|] => /=.
+    iApply sim_tgt_state_transform; [done|] => /=.
     iApply (sim_tgt_map with "[-]").
     iApply sim_tgt_seq_product_None. iIntros (p) "!>". iIntros (????).
     inv_all @link_filter.
     iApply (bi_mono1_intro with "[HΠ]"); [by iApply "HΠ"|] => /=.
     iIntros (?) "?". iIntros ([[[??]?]?] ?); simplify_eq/=. by repeat case_match; simplify_eq/=.
-  Admitted.
+  Qed.
 
   Definition link_tgt_left_handler R (m1 m2 : mod_trans (io_event EV))
     (Π : option (io_event EV) → ((link_case EV * S * m_state m1 * m_state m2 → iProp Σ) → iProp Σ) → iProp Σ)
@@ -428,7 +284,7 @@ Section link.
   Proof.
     iIntros "Hsim".
     iApply (sim_tgt_bi_mono1 with "[-]").
-    iApply sim_tgt_state_transform; [naive_solver| admit |done|] => /=.
+    iApply sim_tgt_state_transform; [done|] => /=.
     iApply (sim_tgt_map with "[-]").
     iApply sim_tgt_seq_product_left.
     iApply (sim_tgt_bi_mono2 with "[-]").
@@ -441,7 +297,32 @@ Section link.
     - iApply (bi_mono1_intro with "[Hsim]"); [by iApply "Hsim"|].
       iIntros (?) "HP". iApply (bi_mono1_intro with "HP").
       iIntros (?) "?". iIntros ([[[??]?]?]?). simplify_eq/=. done.
-  Admitted.
+  Qed.
+
+  Lemma sim_tgt_link_left_recv R m1 m2 s σ1 σ2 Π e :
+    (σ1 ≈{m1}≈>ₜ λ κ Pσ,
+      match κ with
+      | None => Π None (λ P, Pσ (λ σ1', P (MLFRecvL e, s, σ1', σ2)))
+      | Some e' => ⌜e' = (Incoming, e)⌝ -∗ Π None (λ P, Pσ (λ σ1', P (MLFLeft, s, σ1', σ2)))
+      end%I) -∗
+    (MLFRecvL e, s, σ1, σ2) ≈{link_trans R m1 m2}≈>ₜ Π.
+  Proof.
+    iIntros "Hsim".
+    iApply (sim_tgt_bi_mono1 with "[-]").
+    iApply sim_tgt_state_transform; [done|] => /=.
+    iApply (sim_tgt_map with "[-]").
+    iApply sim_tgt_seq_product_left.
+    iApply (sim_tgt_bi_mono2 with "[-]").
+    iApply (sim_tgt_wand with "Hsim").
+    iIntros (κ ?) "Hsim". iIntros (??????). destruct κ; destruct!/=.
+    - inv_all @link_filter.
+      iApply (bi_mono1_intro with "[Hsim]"); [by iApply "Hsim"|].
+      iIntros (?) "HP". iApply (bi_mono1_intro with "HP").
+      iIntros (?) "?". iIntros ([[[??]?]?]?). by simplify_eq/=.
+    - iApply (bi_mono1_intro with "[Hsim]"); [by iApply "Hsim"|].
+      iIntros (?) "HP". iApply (bi_mono1_intro with "HP").
+      iIntros (?) "?". iIntros ([[[??]?]?]?). simplify_eq/=. done.
+  Qed.
 End link.
 
 Program Definition spec_mod_lang {Σ} (EV S : Type) (state_interp : S → iProp Σ)  : mod_lang EV Σ := {|
@@ -518,11 +399,7 @@ Section spec.
   Qed.
 
   Lemma sim_src_TVis k Π Φ e :
-    (∀ σ,
-        (∀ Π',
-            SRC k tt [{ Π' }] {{ Φ }} -∗
-            σ ≈{spec_trans EV S}≈>ₛ Π') -∗
-     Π (Some e) σ) -∗
+    (∀ σ, σ ⤇ₛ (λ Π, SRC k tt [{ Π }] {{ Φ }}) -∗ Π (Some e) σ) -∗
     SRC (Spec.bind (TVis e) k) [{ Π }] {{ Φ }}.
   Proof.
     iIntros "Hsim". rewrite unfold_bind/=. setoid_rewrite unfold_bind; simpl.
@@ -541,14 +418,14 @@ Section memmove.
 
   Context `{!dimsumGS Σ} `{!recGS Σ}.
   Lemma memmove_sim  :
-    rec_fn_auth (main_prog ∪ memmove_prog ∪ memcpy_prog) -∗
-      (MLFNone, [], rec_init (main_prog ∪ memmove_prog ∪ memcpy_prog), (locle_spec, ())) ⪯{
-        rec_link_trans {["main"; "memmove"; "memcpy"]} {["locle"]} rec_trans (spec_trans rec_event ()),
-        spec_trans rec_event ()} (main_spec, ()).
+    rec_state_interp (rec_init (main_prog ∪ memmove_prog ∪ memcpy_prog)) -∗
+    (MLFNone, [], rec_init (main_prog ∪ memmove_prog ∪ memcpy_prog), (locle_spec, ())) ⪯{
+      rec_link_trans {["main"; "memmove"; "memcpy"]} {["locle"]} rec_trans (spec_trans rec_event ()),
+      spec_trans rec_event ()} (main_spec, ()).
   Proof.
-    iIntros "?". iApply (sim_tgt_handler_intro with "[-]").
-    iApply (sim_tgt_link_None with "[-]"). iIntros "!>" (??????). destruct!/=.
-    case_match; destruct!/=.
+    iIntros "Hstate". iApply (sim_tgt_handler_intro with "[-]").
+    iApply (sim_tgt_link_None with "[-]").
+    iIntros "!>" (??????). destruct!/=. case_match; destruct!/=.
     unfold sim_tgt_handler.
     iApply (sim_src_expr_elim with "[] [-]"); [simpl; done..|].
     rewrite /main_spec/TReceive bind_bind.
@@ -560,6 +437,10 @@ Section memmove.
     iApply sim_src_TAssume. iIntros (?).
     iApply sim_src_TAssume. iIntros (?). simplify_eq.
     rewrite bool_decide_true; [|done].
+    iApply sim_src_expr_stop1. iIntros (?) "Hsrc". iSplit!.
+    iApply (sim_tgt_handler_intro with "[-]").
+    iApply (sim_tgt_link_left_recv with "[-]").
+    iApply (sim_tgt_expr_elim [] (_ @ _) with "Hstate [-]"); [done|] => /=.
     (* iApply sim_src_expr_stop. *)
   Admitted.
 End memmove.
@@ -572,8 +453,10 @@ Lemma memmove_refines_spec :
 Proof.
   apply (sim_adequacy #[dimsumΣ; recΣ]); [apply _..|].
   iIntros (??) "!>". simpl.
-  iApply memmove_sim.
-Abort.
+  iApply (fupd_sim with "[-]").
+  iMod recgs_alloc as (?) "[?[??]]". iModIntro.
+  iApply memmove_sim. iFrame.
+Qed.
 
 (* Idea: construct PI for source level proof from pre and
 postconditions of all the external functions instead of constructing
