dimsum/iris/combinators.v
@@ -1,0 +1,326 @@
+From dimsum.core Require Import product seq_product state_transform.
+From dimsum.core.iris Require Export sim.
+Set Default Proof Using "Type".
+
+(** * map_mod *)
+
+Section map.
+  Context {Σ : gFunctors} {EV1 EV2 : Type} {S : Type} `{!dimsumGS Σ}.
+  Implicit Types (f : map_mod_fn EV1 EV2 S).
+
+  Lemma sim_tgt_map m f σ σf Π :
+    (σ ≈{m}≈>ₜ λ κ Pσ,
+      ∀ κ' σf' ok, ⌜if κ is Some e then f σf e κ' σf' ok else κ' = None ∧ σf' = σf ∧ ok = true⌝ -∗
+         Π κ' (λ P, Pσ (λ σ', P (σ', (σf', ok))))) -∗
+    (σ, (σf, true)) ≈{map_trans m f}≈>ₜ Π.
+  Proof.
+    iIntros "Hsim".
+    pose (F := (λ σ Π', (∀ κ Pσ, Π' κ Pσ -∗
+         ∀ κ' σf' ok, ⌜if κ is Some e then f σf e κ' σf' ok else κ' = None ∧ σf' = σf ∧ ok = true⌝ -∗
+          Π κ' (λ P, Pσ (λ σ', P (σ', (σf', ok))))) -∗ (σ, (σf, true)) ≈{map_trans m f}≈>ₜ Π)%I).
+    iAssert (∀ Π, σ ≈{ m }≈>ₜ Π -∗ F σ Π)%I as "Hgen"; last first.
+    { iApply ("Hgen" with "Hsim"). iIntros (??) "?". done. }
+    iIntros (?) "Hsim".
+    iApply (sim_tgt_ind with "[] Hsim"). { solve_proper. }
+    iIntros "!>" (??) "Hsim". iIntros "Hc".
+    iApply (sim_tgt_ctx with "[-]"). iIntros "?".
+    iApply (sim_tgt_bi_mono1 with "[-]").
+    iApply (fupd_sim_tgt with "[-]").
+    iMod ("Hsim" with "[$]") as "[[% [? HP]]| Hs ]". {
+      iModIntro. iDestruct ("Hc" with "[$] [//]") as "Hc".
+      iApply (sim_tgt_stop with "[-]").
+      iApply (bi_mono1_intro with "Hc"). iIntros (?) "?".
+      iDestruct ("HP" with "[$]") as "$".
+    }
+    iModIntro. iApply (sim_tgt_step with "[-]"). iIntros (?? Hstep). inv_all/= @m_step.
+    all: iMod ("Hs" with "[//]") as "Hs"; do 2 iModIntro.
+    - do 2 case_match; simplify_eq. iDestruct "Hs" as "[[% [? HP]]|[%[%[% HF]]]]".
+      + iDestruct ("Hc" with "[$] [//]") as "Hc".
+        iLeft. iApply (bi_mono1_intro with "Hc"). iIntros (?) "?".
+        iDestruct ("HP" with "[$]") as (??) "?".
+        iExists (_, _). iFrame. iSplit!.
+      + iRight. iExists (_, _). iSplit!; [done|].
+        iApply (sim_tgt_wand with "[-] []"); [by iApply "HF"|].
+        iIntros (??) "HΠ". by iApply bi_mono1_intro0.
+    - iDestruct "Hs" as "[[% [? HP]]|[%[%[% HF]]]]"; simplify_eq.
+      iDestruct ("Hc" with "[$] [//]") as "Hc".
+      iLeft. iExists _. iFrame. iIntros (?) "?".
+      iDestruct ("HP" with "[$]") as (??) "?".
+      iExists (_, _). iFrame. iSplit!.
+  Qed.
+
+  Lemma sim_src_map m f σ σf Π `{!VisNoAng m} :
+    (σ ≈{m}≈>ₛ λ κ σ',
+      ∃ κ' σf' ok, ⌜if κ is Some e then f σf e κ' σf' ok else κ' = None ∧ σf' = σf ∧ ok = true⌝ ∗
+         Π κ' (σ', (σf', ok))) -∗
+    (σ, (σf, true)) ≈{map_trans m f}≈>ₛ Π.
+  Proof.
+    iIntros "Hsim".
+    pose (F := (λ σ Π', (∀ κ σ', Π' κ σ' -∗
+         ∃ κ' σf' ok, ⌜if κ is Some e then f σf e κ' σf' ok else κ' = None ∧ σf' = σf ∧ ok = true⌝ ∗
+          Π κ' (σ', (σf', ok))) -∗ (σ, (σf, true)) ≈{map_trans m f}≈>ₛ Π)%I).
+    iAssert (∀ Π, σ ≈{ m }≈>ₛ Π -∗ F σ Π)%I as "Hgen"; last first.
+    { iApply ("Hgen" with "Hsim"). iIntros (??) "?". done. }
+    iIntros (?) "Hsim".
+    iApply (sim_src_ind with "[] Hsim"). { solve_proper. }
+    iIntros "!>" (??) "Hsim". iIntros "Hc".
+    iApply (sim_src_ctx with "[-]"). iIntros "?".
+    iApply (fupd_sim_src with "[-]").
+    iMod ("Hsim" with "[$]") as "[?| [%κ [% [% Hs]]] ]". {
+      iModIntro. iApply (sim_src_stop with "[-]").
+      iDestruct ("Hc" with "[$]") as (???[?[??]]) "Hc". by simplify_eq.
+    }
+    destruct κ.
+    - exploit vis_no_all; [done|] => -[σ'' ?].
+      iMod ("Hs" with "[%]") as "Hs"; [naive_solver|]. iModIntro.
+      iDestruct ("Hc" with "[$]") as (????) "Hs".
+      iApply (sim_src_step_end with "[-]"). { econs. { apply: ProductStepBoth; [done|]. by econs. } done. }
+      iIntros ([σ' ?] [??]) "!>". have ? : σ' = σ'' by naive_solver. by simplify_eq.
+    - iModIntro. iApply (sim_src_step with "[-]"). { econs; [by econs|done]. }
+      iIntros ([??][??]). simplify_eq. iMod ("Hs" with "[//]") as "HF". iModIntro.
+      by iApply "HF".
+  Qed.
+
+  Lemma sim_src_map_ub m f σ σf Π `{!VisNoAng m} :
+    ⊢ (σ, (σf, false)) ≈{map_trans m f}≈>ₛ Π.
+  Proof.
+    iStartProof. iApply sim_src_step. { econs. { by apply: ProductStepR; econs. } done. }
+    iIntros ([??] [??]). done.
+  Qed.
+End map.
+
+(** * seq_product *)
+
+Section seq_product.
+  Context {Σ : gFunctors} {EV : Type} `{!dimsumGS Σ}.
+
+  Lemma sim_tgt_seq_product_None (m1 m2 : mod_trans EV) σ1 σ2 Π :
+    (∀ p, ▷ₒ Π (Some (SPENone p)) (λ P, P (p, σ1, σ2))) -∗
+    (SPNone, σ1, σ2) ≈{seq_product_trans m1 m2}≈>ₜ Π.
+  Proof.
+    iIntros "HΠ". iApply (sim_tgt_bi_mono with "[-]").
+    iApply (sim_tgt_step_end with "[-]"). iIntros (???). inv_all @m_step. iSpecialize ("HΠ" $! _).
+    do 2 iModIntro. iApply (bi_mono1_intro with "HΠ"). iIntros (?) "?".
+    iApply bi_mono1_intro0. iSplit!.
+  Qed.
+
+  Lemma sim_tgt_seq_product_left (m1 m2 : mod_trans EV) σ1 σ2 Π :
+    (σ1 ≈{m1}≈>ₜ λ κ Pσ,
+      ∀ s', ⌜if κ is None then s' = SPLeft else True⌝ -∗
+         Π ((λ e, SPELeft e s') <$> κ) (λ P, Pσ (λ σ', P (s', σ', σ2)))) -∗
+    (SPLeft, σ1, σ2) ≈{seq_product_trans m1 m2}≈>ₜ Π.
+  Proof.
+    iIntros "Hsim".
+    pose (F := (λ σ Π', (∀ κ Pσ, Π' κ Pσ -∗
+         ∀ s', ⌜if κ is None then s' = SPLeft else True⌝ -∗
+         Π ((λ e, SPELeft e s') <$> κ) (λ P, Pσ (λ σ', P (s', σ', σ2)))) -∗
+         (SPLeft, σ, σ2) ≈{seq_product_trans m1 m2}≈>ₜ Π)%I).
+    iAssert (∀ Π, σ1 ≈{ m1 }≈>ₜ Π -∗ F σ1 Π)%I as "Hgen"; last first.
+    { iApply ("Hgen" with "Hsim"). iIntros (??) "?". done. }
+    iIntros (?) "Hsim".
+    iApply (sim_tgt_ind with "[] Hsim"). { solve_proper. }
+    iIntros "!>" (??) "Hsim". iIntros "Hc".
+    iApply (sim_tgt_ctx with "[-]"). iIntros "?".
+    iApply (sim_tgt_bi_mono1 with "[-]").
+    iApply (fupd_sim_tgt with "[-]").
+    iMod ("Hsim" with "[$]") as "[[% [? HP]]| Hs ]". {
+      iModIntro. iDestruct ("Hc" with "[$] [//]") as "Hc".
+      iApply sim_tgt_stop.
+      iApply (bi_mono1_intro with "[Hc] [-]"); [done|].
+      iIntros (?) "?". by iDestruct ("HP" with "[$]") as "HP".
+    }
+    iModIntro. iApply (sim_tgt_step with "[-]"). iIntros (?? Hstep). inv_all/= @m_step.
+    iMod ("Hs" with "[//]") as "Hs"; do 2 iModIntro.
+    iDestruct "Hs" as "[[% [? HP]]|[%[%[% HF]]]]"; simplify_eq/=.
+    - iDestruct ("Hc" with "[$] [//]") as "Hc".
+      iLeft. iApply (bi_mono1_intro with "Hc").
+      iIntros (?) "?".
+      iDestruct ("HP" with "[$]") as (??) "?".
+      iExists (_, _, _). iSplit!; [done|]. by iFrame.
+    - iRight. iExists (_, _, _). iSplit!; [done|].
+      iApply (sim_tgt_wand with "[-] []"); [by iApply "HF"|].
+      iIntros (??) "HΠ". by iApply bi_mono1_intro0.
+  Qed.
+
+  Lemma sim_tgt_seq_product_right (m1 m2 : mod_trans EV) σ1 σ2 Π :
+    (σ2 ≈{m2}≈>ₜ λ κ Pσ,
+      ∀ s', ⌜if κ is None then s' = SPRight else True⌝ -∗
+         Π ((λ e, SPERight e s') <$> κ) (λ P, Pσ (λ σ', P (s', σ1, σ')))) -∗
+    (SPRight, σ1, σ2) ≈{seq_product_trans m1 m2}≈>ₜ Π.
+  Proof.
+    iIntros "Hsim".
+    pose (F := (λ σ Π', (∀ κ Pσ, Π' κ Pσ -∗
+         ∀ s', ⌜if κ is None then s' = SPRight else True⌝ -∗
+         Π ((λ e, SPERight e s') <$> κ) (λ P, Pσ (λ σ', P (s', σ1, σ')))) -∗
+         (SPRight, σ1, σ) ≈{seq_product_trans m1 m2}≈>ₜ Π)%I).
+    iAssert (∀ Π, σ2 ≈{ m2 }≈>ₜ Π -∗ F σ2 Π)%I as "Hgen"; last first.
+    { iApply ("Hgen" with "Hsim"). iIntros (??) "?". done. }
+    iIntros (?) "Hsim".
+    iApply (sim_tgt_ind with "[] Hsim"). { solve_proper. }
+    iIntros "!>" (??) "Hsim". iIntros "Hc".
+    iApply (sim_tgt_ctx with "[-]"). iIntros "?".
+    iApply (sim_tgt_bi_mono1 with "[-]").
+    iApply (fupd_sim_tgt with "[-]").
+    iMod ("Hsim" with "[$]") as "[[% [? HP]]| Hs ]". {
+      iModIntro. iDestruct ("Hc" with "[$] [//]") as "Hc".
+      iApply sim_tgt_stop.
+      iApply (bi_mono1_intro with "[Hc] [-]"); [done|].
+      iIntros (?) "?". by iDestruct ("HP" with "[$]") as "HP".
+    }
+    iModIntro. iApply (sim_tgt_step with "[-]"). iIntros (?? Hstep). inv_all/= @m_step.
+    iMod ("Hs" with "[//]") as "Hs"; do 2 iModIntro.
+    iDestruct "Hs" as "[[% [? HP]]|[%[%[% HF]]]]"; simplify_eq/=.
+    - iDestruct ("Hc" with "[$] [//]") as "Hc".
+      iLeft. iApply (bi_mono1_intro with "Hc").
+      iIntros (?) "?".
+      iDestruct ("HP" with "[$]") as (??) "?".
+      iExists (_, _, _). iSplit!; [done|]. by iFrame.
+    - iRight. iExists (_, _, _). iSplit!; [done|].
+      iApply (sim_tgt_wand with "[-] []"); [by iApply "HF"|].
+      iIntros (??) "HΠ". by iApply bi_mono1_intro0.
+  Qed.
+
+  Lemma sim_src_seq_product_None p (m1 m2 : mod_trans EV) σ1 σ2 Π :
+    Π (Some (SPENone p)) (p, σ1, σ2) -∗
+    (SPNone, σ1, σ2) ≈{seq_product_trans m1 m2}≈>ₛ Π.
+  Proof.
+    iIntros "HΠ". iApply (sim_src_step_end with "[-]"); [by econs|].
+    iIntros (??). by simplify_eq.
+  Qed.
+
+  Lemma sim_src_seq_product_left (m1 m2 : mod_trans EV) σ1 σ2 Π `{!VisNoAng m1} :
+    (σ1 ≈{m1}≈>ₛ λ κ σ', ∃ s', ⌜if κ is None then s' = SPLeft else True⌝ ∗
+       Π ((λ e, SPELeft e s') <$> κ) (s', σ', σ2)) -∗
+    (SPLeft, σ1, σ2) ≈{seq_product_trans m1 m2}≈>ₛ Π.
+  Proof.
+    iIntros "Hsim".
+    pose (F := (λ σ Π', (∀ κ σ, Π' κ σ -∗
+         ∃ s', ⌜if κ is None then s' = SPLeft else True⌝ ∗
+         Π ((λ e, SPELeft e s') <$> κ) (s', σ, σ2)) -∗
+         (SPLeft, σ, σ2) ≈{seq_product_trans m1 m2}≈>ₛ Π)%I).
+    iAssert (∀ Π, σ1 ≈{ m1 }≈>ₛ Π -∗ F σ1 Π)%I as "Hgen"; last first.
+    { iApply ("Hgen" with "Hsim"). iIntros (??) "?". done. }
+    iIntros (?) "Hsim".
+    iApply (sim_src_ind with "[] Hsim"). { solve_proper. }
+    iIntros "!>" (??) "Hsim". iIntros "Hc".
+    iApply (sim_src_ctx with "[-]"). iIntros "?".
+    iApply (fupd_sim_src with "[-]").
+    iMod ("Hsim" with "[$]") as "[?| [%κ [% [% Hsim]]] ]". {
+      iModIntro. iDestruct ("Hc" with "[$]") as (??) "Hc".
+      iApply (sim_src_stop with "[-]"). by simplify_eq/=.
+    }
+    destruct κ.
+    - exploit vis_no_all; [done|] => -[σs1 ?].
+      iMod ("Hsim" with "[%]") as "?"; [naive_solver|].
+      iDestruct ("Hc" with "[$]") as (s ?) "?".
+      iApply (sim_src_step with "[-]"). { by apply: (SPLeftS _ _ _ _ _ s). }
+      iIntros ([[? σs2]?] [?[??]]). have ? : σs1 = σs2 by naive_solver. by simplify_eq/=.
+    - iModIntro. iApply (sim_src_step with "[-]"). { by econs. }
+      iIntros ([[??] ?] [?[??]]). simplify_eq.
+      iMod ("Hsim" with "[//]") as "Hsim". iModIntro. by iApply "Hsim".
+  Qed.
+
+  Lemma sim_src_seq_product_right (m1 m2 : mod_trans EV) σ1 σ2 Π `{!VisNoAng m2} :
+    (σ2 ≈{m2}≈>ₛ λ κ σ', ∃ s', ⌜if κ is None then s' = SPRight else True⌝ ∗
+       Π ((λ e, SPERight e s') <$> κ) (s', σ1, σ')) -∗
+    (SPRight, σ1, σ2) ≈{seq_product_trans m1 m2}≈>ₛ Π.
+  Proof.
+    iIntros "Hsim".
+    pose (F := (λ σ Π', (∀ κ σ, Π' κ σ -∗
+         ∃ s', ⌜if κ is None then s' = SPRight else True⌝ ∗
+         Π ((λ e, SPERight e s') <$> κ) (s', σ1, σ)) -∗
+         (SPRight, σ1, σ) ≈{seq_product_trans m1 m2}≈>ₛ Π)%I).
+    iAssert (∀ Π, σ2 ≈{ m2 }≈>ₛ Π -∗ F σ2 Π)%I as "Hgen"; last first.
+    { iApply ("Hgen" with "Hsim"). iIntros (??) "?". done. }
+    iIntros (?) "Hsim".
+    iApply (sim_src_ind with "[] Hsim"). { solve_proper. }
+    iIntros "!>" (??) "Hsim". iIntros "Hc".
+    iApply (sim_src_ctx with "[-]"). iIntros "?".
+    iApply (fupd_sim_src with "[-]").
+    iMod ("Hsim" with "[$]") as "[?| [%κ [% [% Hsim]]] ]". {
+      iModIntro. iDestruct ("Hc" with "[$]") as (??) "Hc".
+      iApply (sim_src_stop with "[-]"). by simplify_eq/=.
+    }
+    destruct κ.
+    - exploit vis_no_all; [done|] => -[σs1 ?].
+      iMod ("Hsim" with "[%]") as "?"; [naive_solver|].
+      iDestruct ("Hc" with "[$]") as (s ?) "?".
+      iApply (sim_src_step with "[-]"). { by apply: (SPRightS _ _ _ _ _ s). }
+      iIntros ([[? ?]σs2] [?[??]]). have ? : σs1 = σs2 by naive_solver. by simplify_eq/=.
+    - iModIntro. iApply (sim_src_step with "[-]"). { by econs. }
+      iIntros ([[??] ?] [?[??]]). simplify_eq.
+      iMod ("Hsim" with "[//]") as "Hsim". iModIntro. by iApply "Hsim".
+  Qed.
+End seq_product.
+
+
+(** * state_transform_mod *)
+
+Section state_transform.
+  Context {Σ : gFunctors} {EV : Type} {S : Type} `{!dimsumGS Σ}.
+
+  Lemma sim_tgt_state_transform (m : mod_trans EV) σ' (R : S → m.(m_state) → Prop) σ Π `{!StateTransformWf m R} :
+   R σ σ' →
+   (σ' ≈{m}≈>ₜ λ κ Pσ, Π κ (λ P, Pσ (λ σ'', ∀ σ''', ⌜R σ''' σ''⌝ -∗ P σ'''))) -∗
+    σ ≈{state_transform_trans m R}≈>ₜ Π.
+  Proof.
+    destruct StateTransformWf0 as [Heq HRstep].
+    iIntros (HR) "Hsim".
+    pose (F := (λ σ' Π', ∀ σ,
+                   ⌜R σ σ'⌝ -∗
+                   (∀ κ Pσ, Π' κ Pσ -∗ Π κ (λ P, Pσ (λ σ'', ∀ σ''', ⌜R σ''' σ''⌝ -∗ P σ'''))) -∗
+                   σ ≈{state_transform_trans m R}≈>ₜ Π)%I).
+    iAssert (∀ Π, σ' ≈{ m }≈>ₜ Π -∗ F σ' Π)%I as "Hgen"; last first.
+    { iApply ("Hgen" with "Hsim"); [done|]. iIntros (??) "?". done. }
+    iIntros (?) "Hsim".
+    iApply (sim_tgt_ind with "[] Hsim"). { solve_proper. }
+    clear σ' σ HR. iIntros "!>" (σ'?) "Hsim". iIntros (σ HR) "Hc".
+    iApply (sim_tgt_ctx with "[-]"). iIntros "?".
+    iApply (sim_tgt_bi_mono1 with "[-]").
+    iApply (fupd_sim_tgt with "[-]").
+    iMod ("Hsim" with "[$]") as "[[% [HΠ HP]]| Hs ]". {
+      iModIntro. iApply (sim_tgt_stop with "[-]").
+      iApply (bi_mono1_intro with "[Hc HΠ]"); [by iApply "Hc"|] => /=.
+      iIntros (?) "?". iDestruct ("HP" with "[$]") as "HP". by iApply "HP".
+    }
+    iModIntro. iApply (sim_tgt_step with "[-]"). iIntros (?? Hstep). inv_all/= @m_step.
+    have ?: σ' = σ'0 by naive_solver. subst.
+    iMod ("Hs" with "[//]") as "Hs"; do 2 iModIntro.
+    iDestruct "Hs" as "[[% [? HP]]|[%[%[% HF]]]]".
+    - iDestruct ("Hc" with "[$]") as "Hc".
+      iLeft. iApply (bi_mono1_intro with "Hc"). iIntros (?) "?".
+      iDestruct ("HP" with "[$]") as (??) "HP".
+      exploit HRstep; [done..|] => -[??].
+      iSplit!; [done..|]. by iApply "HP".
+    - iRight. simplify_eq. exploit HRstep; [done..|] => -[??].
+      iSplit!; [done..|]. iApply (sim_tgt_wand with "[-] []"); [by iApply "HF"|].
+      iIntros (??) "HΠ". by iApply bi_mono1_intro0.
+  Qed.
+
+  Lemma sim_src_state_transform (m : mod_trans EV) σ' (R : S → m.(m_state) → Prop) σ Π :
+   R σ σ' →
+   (σ' ≈{m}≈>ₛ λ κ σ'', ∀ σ''', ⌜R σ''' σ''⌝ -∗ Π κ σ''') -∗
+    σ ≈{state_transform_trans m R}≈>ₛ Π.
+  Proof.
+    iIntros (HR) "Hsim".
+    pose (F := (λ σ' Π', ∀ σ,
+                   ⌜R σ σ'⌝ -∗
+                   (∀ κ σ'', Π' κ σ'' -∗ ∀ σ''', ⌜R σ''' σ''⌝ -∗ Π κ σ''') -∗
+                   σ ≈{state_transform_trans m R}≈>ₛ Π)%I).
+    iAssert (∀ Π, σ' ≈{ m }≈>ₛ Π -∗ F σ' Π)%I as "Hgen"; last first.
+    { iApply ("Hgen" with "Hsim"); [done|]. iIntros (??) "?". done. }
+    iIntros (?) "Hsim".
+    iApply (sim_src_ind with "[] Hsim"). { solve_proper. }
+    clear σ' σ HR. iIntros "!>" (σ'?) "Hsim". iIntros (σ HR) "Hc".
+    iApply (sim_src_ctx with "[-]"). iIntros "?".
+    iApply (fupd_sim_src with "[-]").
+    iMod ("Hsim" with "[$]") as "[?| [%κ [% [% Hs]]] ]". {
+      iModIntro. iApply (sim_src_stop with "[-]"). by iApply ("Hc" with "[$]").
+    }
+    iModIntro. iApply (sim_src_step with "[-]"); [by econs|].
+    iIntros (? [?[??]]). iMod ("Hs" with "[//]") as "Hs". iModIntro.
+    case_match.
+    - by iApply ("Hc" with "Hs").
+    - by iApply ("Hs" with "[//]").
+  Qed.
+End state_transform.
